complete ex2

theories/opt/ex2.v
@@ -1,16 +1,16 @@
-From stbor.sim Require Import local invariant refl_step.
+From stbor.sim Require Import local invariant refl tactics simple program
+  refl_step right_step left_step viewshift derived_step.
 
 Set Default Proof Using "Type".
 
 (** Moving read of shared ref up across code that *may* use that ref. *)
 
 (* Assuming x : & i32 *)
-Definition ex2 : function :=
+Definition ex2_unopt : function :=
   fun: ["i"],
     let: "x" := new_place (& int) "i" in
     retag_place "x" (RefPtr Immutable) int Default ;;
-    Copy *{int} "x" ;;
-    Call #[ScFnPtr "f"] ["x"] ;;
+    Call #[ScFnPtr "f"] [Copy "x"] ;;
     let: "v" := Copy *{int} "x" in
     Free "x" ;; Free "i" ;;
     "v"
@@ -20,13 +20,118 @@ Definition ex2_opt : function :=
   fun: ["i"],
     let: "x" := new_place (& int) "i" in
     retag_place "x" (RefPtr Immutable) int Default ;;
-    Copy *{int} "x" ;;
     let: "v" := Copy *{int} "x" in
-    Call #[ScFnPtr "f"] ["x"] ;;
+    Call #[ScFnPtr "f"] [Copy "x"] ;;
     Free "x" ;; Free "i" ;;
     "v"
   .
 
-Lemma ex2_sim_body : ⊨ᶠ ex2 ≥ ex2_opt.
+Lemma ex2_sim_body : ⊨ᶠ ex2_unopt ≥ ex2_opt.
 Proof.
-Abort.
+  apply (sim_fun_simple1 10)=>// fs ft rarg es et arg c LOOK AREL ??.
+  simplify_eq/=.
+  (* Alloc local *)
+  sim_apply sim_simple_alloc_local=> l t /=.
+  sim_apply sim_simple_let=>/=.
+  (* Write local *)
+  sim_apply sim_simple_write_local; [solve_sim..|].
+  intros sarg ->.
+  sim_apply sim_simple_let=>/=.
+  apply: sim_simple_result.
+  (* Retag a local place *)
+  sim_apply sim_simple_let=>/=.
+  apply Forall2_cons_inv in AREL as [AREL _].
+  (* We need to drop to complex mode, to preserve some local state info. *)
+  intros σs σt.
+  sim_apply sim_body_let=>/=.
+    (* Copy local place *)
+    sim_apply sim_body_copy_local; [solve_sim..|].
+    sim_apply sim_body_result. simpl. intros VALID.
+    (* Retag *)
+    sim_apply sim_body_retag_ref_default; [simpl; lia|done| |eauto|..].
+    { eapply arel_mono; [done|..|exact AREL]. solve_res. } clear VALID.
+    move=> l' told tnew hplt c' cids α' nxtp' ? _ _ IS_i σs' σt' s_new
+      tk ARELn /=. subst sarg.
+    specialize (IS_i O ltac:(simpl; lia)). rewrite shift_loc_0_nat in IS_i.
+    destruct IS_i as [[[ss st] IS_i] TOP].
+    (* Write local *)
+    sim_apply sim_body_write_local_1; [solve_sim..|].
+    intros s ?. simplify_eq. simpl.
+  sim_apply sim_body_let. simplify_eq/=.
+  (* Copy local (right) *)
+  sim_apply_r sim_body_copy_local_r; [solve_sim..|].
+  apply: sim_body_result=>_. simpl.
+  (* Copy public right *)
+  sim_apply_r sim_body_deref_r. simpl.
+  sim_apply_r sim_body_copy_SRO_public_r; [solve_sim..|].
+  apply: sim_body_result=>_. simpl.
+  apply: sim_body_let_r. simpl.
+  (* Back to simple mode! *)
+  eapply (sim_simplify (fun_post_simple c)). { by eauto. }
+  simplify_eq/=.
+  (* Copy local *)
+  sim_apply sim_simple_copy_local; [solve_sim..|].
+  apply: sim_simple_result. simpl.
+  (* Call *)
+  rewrite (_: rarg ⋅ res_cs c ∅ ⋅ res_tag tnew tk hplt ⋅
+                res_loc l [(ScPtr l' (Tagged tnew), ScPtr l' (Tagged tnew))] t
+              ≡ rarg ⋅ res_cs c ∅ ⋅ res_tag tnew tk hplt ⋅
+                res_loc l [(ScPtr l' (Tagged tnew), ScPtr l' (Tagged tnew))] t ⋅
+                res_tag tnew tk hplt); last first.
+  { rewrite {1}res_tag_public_dup cmra_assoc. solve_res. }
+  sim_apply (sim_simple_call 5 [ValR [ScPtr l' (Tagged tnew)]]
+                               [ValR [ScPtr l' (Tagged tnew)]]
+              (res_tag tnew tkPub hplt)); [solve_sim..| |].
+  { constructor; [|by constructor].
+    constructor; [done|by constructor]. } clear ARELn.
+  intros rf' frs' frt' ??? ? _ _ FREL'. simplify_eq/=.
+  apply: sim_simple_result. simpl.
+  sim_apply sim_simple_let=>/=. clear σs' σt' nxtp' α' TOP σs σt.
+  (* Copy local (left). We drop to complex just because simple does not support this yet. *)
+  intros σs σt.
+  sim_apply_l sim_body_copy_local_l; [solve_sim..|].
+  apply: sim_body_result=>_. simpl.
+  (* Copy public (left) *)
+  sim_apply_l sim_body_deref_l. simpl.
+  sim_apply_l sim_body_copy_public_l; [try solve_sim..|].
+  intros r' AREL'.
+  apply: sim_body_result=>Hval. simpl.
+  apply: sim_body_let_l. simpl.
+  (* Free stuff *)
+  eapply (sim_simplify (fun_post_simple c)). { by eauto. }
+  sim_apply sim_simple_free_local_1; [solve_sim..|]. simpl.
+  sim_apply sim_simple_let=>/=.
+  sim_apply sim_simple_free_public.
+  { simpl. constructor; [|by constructor].
+    apply: arel_mono; last fast_done.
+    apply: cmra_valid_included; first fast_done.
+    do 2 apply cmra_mono_r. solve_res. solve_res. }
+  sim_apply sim_simple_let=>/=.
+  (* Finishing up. *)
+  apply: sim_simple_result. split.
+  - solve_res.
+  - constructor; simpl; auto.
+    eapply arel_mono; [..|solve_res|exact AREL'].
+    eapply cmra_valid_included; [exact Hval|].
+    do 2 apply cmra_mono_r. solve_res.
+Qed.
+
+(** Top-level theorem: Two programs that only differ in the
+"ex2" function are related. *)
+Corollary ex2 (prog: fn_env) :
+  stuck_decidable →
+  prog_wf prog →
+  let prog_src := <["ex2":=ex2_unopt]> prog in
+  let prog_tgt := <["ex2":=ex2_opt]> prog in
+  behave_prog prog_tgt <1= behave_prog prog_src.
+Proof.
+  intros Hdec Hwf. apply sim_prog_sim_classical.
+  { apply Hdec. }
+  { apply has_main_insert, Hwf; done. }
+  apply sim_mod_funs_local.
+  apply sim_mod_funs_insert; first done.
+  - exact: ex2_sim_body.
+  - exact: sim_mod_funs_refl.
+Qed.
+
+Print Assumptions ex2.
