theories/opt/ex1.v
@@ -51,7 +51,7 @@ Proof.
     apply sim_simple_valid_post.
     apply: sim_simple_result. simpl. intros VALID.
     (* Retag *)
-    sim_apply sim_simple_retag_mut_ref; [simpl; lia| |eauto|..].
+    sim_apply sim_simple_retag_ref; [simpl; lia|done| |eauto|..].
     { eapply arel_mono; [done|..|exact AREL]. solve_res. } clear VALID.
     move=>l_i tg_i tg_n hplt /= ? IS_i. subst sarg.
     specialize (IS_i O ltac:(lia)). rewrite shift_loc_0_nat in IS_i.
