theories/opt/ex1_down.v
@@ -1,4 +1,6 @@
 From stbor.sim Require Import local invariant refl_step.
+From stbor.sim Require Import tactics simple program.
+From stbor.sim Require Import refl_step right_step left_step viewshift.
 
 Set Default Proof Using "Type".
 
@@ -24,7 +26,90 @@ Definition ex1_down_opt : function :=
     Copy *{int} "x"
     .
 
-
 Lemma ex1_down_sim_fun : ⊨ᶠ ex1_down ≥ ex1_down_opt.
 Proof.
+  apply (sim_fun_simple1 10)=>// fs ft rarg es et arg c LOOK AREL ??.
+  simplify_eq/=.
+  (* Alloc local *)
+  sim_apply sim_simple_alloc_local=> l t /=.
+  sim_apply sim_simple_let=>/=.
+  (* Write local *)
+  sim_apply sim_simple_write_local; [solve_sim..|].
+  intros sarg ->.
+  sim_apply sim_simple_let=>/=.
+  apply: sim_simple_result.
+  (* Retag a local place *)
+  sim_apply sim_simple_let=>/=.
+  apply Forall2_cons_inv in AREL as [AREL _].
+  sim_apply sim_simple_let=>/=.
+    (* Copy local place *)
+    sim_apply sim_simple_copy_local; [solve_sim..|].
+    apply sim_simple_valid_post.
+    apply: sim_simple_result. simpl. intros VALID.
+    (* TODO: need a rule to add a tag to res_cs.
+      Also need a rule to remove it at the end. *)
+    (* Retag *)
+    (* sim_apply sim_simple_retag_mut_ref; [simpl; lia| |eauto|..].
+    { eapply arel_mono; [done|..|exact AREL]. solve_res. } clear VALID.
+    move=>l_i tg_i tg_n hplt /= ? IS_i. subst sarg.
+    specialize (IS_i O ltac:(lia)). rewrite shift_loc_0_nat in IS_i.
+    (* Write local *)
+    sim_apply sim_simple_write_local; [solve_sim..|].
+    intros s ?. simplify_eq.
+  (* Call *)
+  sim_apply sim_simple_let=>/=.
+  sim_apply (sim_simple_call 10 [] [] ε); [solve_sim..|].
+  intros rf frs frt ??? ? _ _ FREL. simplify_eq/=.
+  apply: sim_simple_result. simpl.
+  sim_apply sim_simple_let=>/=.
+  (* Copy local *)
+  sim_apply sim_simple_copy_local; [solve_sim..|].
+  apply: sim_simple_result. simpl.
+  sim_apply sim_simple_deref=>l' t' ?. simplify_eq/=.
+  (* Write unique. We need to drop to complex mode, to preserve some local state info. *)
+  intros σs σt.
+  sim_apply sim_body_write_unique_1; [solve_sim..|].
+  intros ?? Htop. simplify_eq/=.
+  sim_apply sim_body_let. simplify_eq/=.
+  (* Copy local (right) *)
+  sim_apply_r sim_body_copy_local_r; [solve_sim..|].
+  apply: sim_body_result=>_. simpl.
+  (* Copy unique (right) *)
+  sim_apply_r sim_body_deref_r. simpl.
+  sim_apply_r sim_body_copy_unique_r; [try solve_sim..|].
+  { rewrite lookup_insert. done. }
+  apply: sim_body_result=>_. simpl.
+  apply: sim_body_let_r. simpl. (* FIXME: figure out why [sim_apply_r] does the wrong thing here *)
+  (* We can go back to simple mode! *)
+  eapply (sim_simplify (fun_post_simple c)). { by eauto. }
+  simplify_eq/=. clear- AREL FREL LOOK.
+  (* Call *)
+  sim_apply (sim_simple_call 10 [] [] ε); [solve_sim..|].
+  intros rf' frs' frt' ??? ? _ _ FREL'. simplify_eq/=.
+  apply: sim_simple_result. simpl.
+  sim_apply sim_simple_let=>/=.
+  (* Copy local (left). We drop to complex just because simple does not support this yet. *)
+  intros σs σt.
+  sim_apply_l sim_body_copy_local_l; [solve_sim..|].
+  apply: sim_body_result=>_. simpl.
+  (* Copy unique (left) *)
+  sim_apply_l sim_body_deref_l. simpl.
+  sim_apply_l sim_body_copy_unique_l; [try solve_sim..|].
+  { rewrite lookup_insert. done. }
+  apply: sim_body_result=>Hval. simpl.
+  apply: sim_body_let_l. simpl.
+  (* Free stuff *)
+  eapply (sim_simplify (fun_post_simple c)). { by eauto. }
+  sim_apply sim_simple_free_local_1; [solve_sim..|]. simpl.
+  sim_apply sim_simple_let=>/=.
+  sim_apply sim_simple_free_public.
+  { simpl. constructor; [|by constructor].
+    apply: arel_mono; last fast_done.
+    apply: cmra_valid_included; first fast_done.
+    do 3 apply cmra_mono_r. solve_res. solve_res. }
+  sim_apply sim_simple_let=>/=.
+  (* Finishing up. *)
+  apply: sim_simple_result. split.
+  - solve_res.
+  - constructor; simpl; auto. *)
 Abort.
