theories/sim/derived_step.v
@@ -1,0 +1,14 @@
+From stbor.sim Require Import left_step right_step.
+
+Lemma sim_body_copy_local fs ft r r' n l t ty ss st σs σt Φ :
+  tsize ty = 1%nat →
+  r ≡ r' ⋅ res_loc l [(ss, st)] t →
+  (r ⊨{n,fs,ft} (#[ss], σs) ≥ (#[st], σt) : Φ) →
+  r ⊨{S n,fs,ft}
+    (Copy (Place l (Tagged t) ty), σs) ≥ (Copy (Place l (Tagged t) ty), σt)
+  : Φ.
+Proof.
+  intros ?? Hcont.
+  eapply sim_body_copy_local_l; [done..|].
+  eapply sim_body_copy_local_r; done.
+Qed.
